Phi_Semantics/PhiSem_CF_Breakable.thy
@@ -9,8 +9,10 @@ definition continue_label :: \<open>brk_label \<Rightarrow> brk_label\<close>
 
 thm brk_scope
 
-declare [[\<phi>display_brk_frame]]
 declare [[\<phi>trace_reasoning]]
+declare distrib_right[assertion_simps]
+thm assertion_simps
+
 
 proc while:
   assumes \<open>\<^bold>p\<^bold>a\<^bold>r\<^bold>a\<^bold>m (X x \<^bold>s\<^bold>u\<^bold>b\<^bold>j x. Inv: invariant x \<and> Guard: cond x)\<close>
@@ -22,21 +24,31 @@ proc while:
                     \<^bold>p\<^bold>r\<^bold>o\<^bold>c Body \<lbrace> X x\<heavy_comma> Brk_Frame (continue_label lc)\<heavy_comma> Brk_Frame lb
                             \<longmapsto> X x'\<heavy_comma> Brk_Frame (continue_label lc)\<heavy_comma> Brk_Frame lb
                                 \<^bold>s\<^bold>u\<^bold>b\<^bold>j x'. invariant x'
-                              \<rbrace> \<^bold>t\<^bold>h\<^bold>r\<^bold>o\<^bold>w\<^bold>s (\<lambda>e. \<^bold>b\<^bold>r\<^bold>e\<^bold>a\<^bold>k lb \<^bold>w\<^bold>i\<^bold>t\<^bold>h (\<lambda>_. X x'\<heavy_comma> Brk_Frame (continue_label lc) \<^bold>s\<^bold>u\<^bold>b\<^bold>j x'. invariant x \<and> \<not> cond x)
-                                         \<^bold>o\<^bold>r \<^bold>b\<^bold>r\<^bold>e\<^bold>a\<^bold>k (continue_label lc) \<^bold>w\<^bold>i\<^bold>t\<^bold>h (\<lambda>_. X x'\<heavy_comma> Brk_Frame lb \<^bold>s\<^bold>u\<^bold>b\<^bold>j x'. invariant x)
+                              \<rbrace> \<^bold>t\<^bold>h\<^bold>r\<^bold>o\<^bold>w\<^bold>s (\<lambda>e. \<^bold>b\<^bold>r\<^bold>e\<^bold>a\<^bold>k lb \<^bold>w\<^bold>i\<^bold>t\<^bold>h (\<lambda>_::unit \<phi>arg. X x'\<heavy_comma> Brk_Frame (continue_label lc) \<^bold>s\<^bold>u\<^bold>b\<^bold>j x'. invariant x' \<and> \<not> cond x')
+                                         \<^bold>o\<^bold>r \<^bold>b\<^bold>r\<^bold>e\<^bold>a\<^bold>k (continue_label lc) \<^bold>w\<^bold>i\<^bold>t\<^bold>h (\<lambda>_::unit \<phi>arg. X x' \<^bold>s\<^bold>u\<^bold>b\<^bold>j x'. invariant x')
                                          \<^bold>o\<^bold>r E2 e)"
   input \<open>U\<close>
   output \<open>X x \<^bold>s\<^bold>u\<^bold>b\<^bold>j x. invariant x \<and> \<not> cond x\<close>
+  throws \<open>E1 + E2\<close>
   \<medium_left_bracket> CT
     brk_scope \<medium_left_bracket> for lb
       PhiSem_CF_Basic.while \<open>Brk_Frame lb\<heavy_comma> X x \<^bold>s\<^bold>u\<^bold>b\<^bold>j x. Inv: invariant x \<and> Guard: cond x\<close>
       \<medium_left_bracket> C \<medium_right_bracket>.
       \<medium_left_bracket> brk_scope \<medium_left_bracket> for lc
-        have wrap: \<open>Brk_Frame lc = Brk_Frame (continue_label lc)\<close> unfolding continue_label_def ..
-        ;; unfold wrap
-           B \<exists>x'
-           fold wrap
-        \<medium_right_bracket>
-        ..
+          B[unfolded continue_label_def, where lb=lb]
+        \<medium_right_bracket> for \<open>(X x'\<heavy_comma> Brk_Frame lb \<^bold>s\<^bold>u\<^bold>b\<^bold>j x'. invariant x')\<heavy_comma> Brk_Frame lc\<close> .. ;;
+      \<medium_right_bracket>. ;;
+    \<medium_right_bracket> for \<open>(X x' \<^bold>s\<^bold>u\<^bold>b\<^bold>j x'. invariant x' \<and> \<not> cond x')\<heavy_comma> Brk_Frame lb\<close> .. ;;
+  \<medium_right_bracket>. .
+
+term \<open>\<^bold>p\<^bold>r\<^bold>o\<^bold>c Body \<lbrace> X x \<longmapsto> \<lambda>\<r>\<e>\<t>. X x' \<^bold>s\<^bold>u\<^bold>b\<^bold>j x'. invariant x' \<rbrace>
+      \<^bold>t\<^bold>h\<^bold>r\<^bold>o\<^bold>w\<^bold>s \<lambda>e. \<^bold>b\<^bold>r\<^bold>e\<^bold>a\<^bold>k lb
+                       \<^bold>w\<^bold>i\<^bold>t\<^bold>h (\<lambda>_. X x'\<heavy_comma> Brk_Frame (continue_label lc) \<^bold>s\<^bold>u\<^bold>b\<^bold>j x'. invariant x' \<and> \<not> cond x')
+                       \<^bold>o\<^bold>r \<^bold>b\<^bold>r\<^bold>e\<^bold>a\<^bold>k (continue_label lc)
+                       \<^bold>w\<^bold>i\<^bold>t\<^bold>h (\<lambda>_. X x' \<^bold>s\<^bold>u\<^bold>b\<^bold>j x'. invariant x')
+                       \<^bold>o\<^bold>r E2 e\<close>
+        thm \<phi>
+
+        term \<open>A \<Longrightarrow> B\<close>
 
 end
