Phi_System/Calculus_of_Programming.thy
@@ -214,8 +214,9 @@ lemma "_\<phi>cast_internal_rule_":
 \<Longrightarrow> \<r>Success
 \<Longrightarrow> \<^bold>o\<^bold>b\<^bold>l\<^bold>i\<^bold>g\<^bold>a\<^bold>t\<^bold>i\<^bold>o\<^bold>n True
 \<Longrightarrow> CurrentConstruction mode blk H T'"
-  unfolding CurrentConstruction_def Action_Tag_def Imply_def FOCUS_TAG_def View_Shift_def
-  by blast
+  unfolding Action_Tag_def
+  using \<phi>apply_view_shift by blast
+
 
 lemma "_\<phi>cast_internal_rule_'":
   " \<^bold>p\<^bold>e\<^bold>n\<^bold>d\<^bold>i\<^bold>n\<^bold>g f \<^bold>o\<^bold>n blk [H] \<^bold>r\<^bold>e\<^bold>s\<^bold>u\<^bold>l\<^bold>t\<^bold>s \<^bold>i\<^bold>n T \<^bold>t\<^bold>h\<^bold>r\<^bold>o\<^bold>w\<^bold>s E
@@ -223,17 +224,15 @@ lemma "_\<phi>cast_internal_rule_'":
 \<Longrightarrow> \<r>Success
 \<Longrightarrow> \<^bold>o\<^bold>b\<^bold>l\<^bold>i\<^bold>g\<^bold>a\<^bold>t\<^bold>i\<^bold>o\<^bold>n True
 \<Longrightarrow> \<^bold>p\<^bold>e\<^bold>n\<^bold>d\<^bold>i\<^bold>n\<^bold>g f \<^bold>o\<^bold>n blk [H] \<^bold>r\<^bold>e\<^bold>s\<^bold>u\<^bold>l\<^bold>t\<^bold>s \<^bold>i\<^bold>n T' \<^bold>t\<^bold>h\<^bold>r\<^bold>o\<^bold>w\<^bold>s E"
-  unfolding Imply_def PendingConstruction_def bind_def Action_Tag_def View_Shift_def
-  by (clarsimp simp add: \<phi>expns LooseStateTy_expn' subset_iff split_state_All)
+  unfolding Action_Tag_def
+  using \<phi>apply_view_shift_pending by blast
 
-(*TODO: \<Longrightarrow> (\<And>v. \<^bold>a\<^bold>r\<^bold>g\<^bold>u\<^bold>m\<^bold>e\<^bold>n\<^bold>t \<^bold>v\<^bold>i\<^bold>e\<^bold>w E v \<longmapsto> E' v)*)
 lemma "_\<phi>cast_exception_":
   " \<^bold>p\<^bold>e\<^bold>n\<^bold>d\<^bold>i\<^bold>n\<^bold>g f \<^bold>o\<^bold>n blk [H] \<^bold>r\<^bold>e\<^bold>s\<^bold>u\<^bold>l\<^bold>t\<^bold>s \<^bold>i\<^bold>n T \<^bold>t\<^bold>h\<^bold>r\<^bold>o\<^bold>w\<^bold>s E
 \<Longrightarrow> (\<And>v. \<^bold>v\<^bold>i\<^bold>e\<^bold>w E v \<longmapsto> E' v @action ToSA)
 \<Longrightarrow> \<^bold>p\<^bold>e\<^bold>n\<^bold>d\<^bold>i\<^bold>n\<^bold>g f \<^bold>o\<^bold>n blk [H] \<^bold>r\<^bold>e\<^bold>s\<^bold>u\<^bold>l\<^bold>t\<^bold>s \<^bold>i\<^bold>n T \<^bold>t\<^bold>h\<^bold>r\<^bold>o\<^bold>w\<^bold>s E'"
-  unfolding Imply_def PendingConstruction_def bind_def View_Shift_def
-  by (clarsimp simp add: \<phi>expns LooseStateTy_expn' subset_iff split_state_All)
-
+  unfolding Action_Tag_def
+  using \<phi>apply_view_shift_pending_E by blast
 
 lemma "_\<phi>cast_exception_rule_":
   " \<^bold>p\<^bold>e\<^bold>n\<^bold>d\<^bold>i\<^bold>n\<^bold>g f \<^bold>o\<^bold>n blk [H] \<^bold>r\<^bold>e\<^bold>s\<^bold>u\<^bold>l\<^bold>t\<^bold>s \<^bold>i\<^bold>n T \<^bold>t\<^bold>h\<^bold>r\<^bold>o\<^bold>w\<^bold>s E
@@ -242,7 +241,6 @@ lemma "_\<phi>cast_exception_rule_":
 \<Longrightarrow> \<^bold>o\<^bold>b\<^bold>l\<^bold>i\<^bold>g\<^bold>a\<^bold>t\<^bold>i\<^bold>o\<^bold>n True
 \<Longrightarrow> \<^bold>p\<^bold>e\<^bold>n\<^bold>d\<^bold>i\<^bold>n\<^bold>g f \<^bold>o\<^bold>n blk [H] \<^bold>r\<^bold>e\<^bold>s\<^bold>u\<^bold>l\<^bold>t\<^bold>s \<^bold>i\<^bold>n T \<^bold>t\<^bold>h\<^bold>r\<^bold>o\<^bold>w\<^bold>s E'"
   using "_\<phi>cast_exception_" .
-
 
 lemma "_\<phi>cast_implication_":
   \<open> \<^bold>a\<^bold>b\<^bold>s\<^bold>t\<^bold>r\<^bold>a\<^bold>c\<^bold>t\<^bold>i\<^bold>o\<^bold>n(x) \<^bold>i\<^bold>s S
