TODO.md
@@ -1,2 +1,3 @@
 - Distance cut in Application reasoning
 - Default attribute for premises
+- Hide scaffolding rules, to optimize sledgeharmer.
